DH example  compute_message1_proof and decode_message1_proof

examples/dh/DY.Example.DH.Protocol.Total.Proof.fst
@@ -6,6 +6,8 @@ open DY.Lib
 open DY.Example.DH.Protocol.Total
 open DY.Example.DH.Protocol.Stateful
 
+#set-options "--fuel 0 --ifuel 0 --z3cliopt 'smt.qi.eager_threshold=100'"
+
 (*** Cryptographic invariants ***)
 
 val dh_crypto_usages: crypto_usages
@@ -33,9 +35,107 @@ let dh_crypto_preds = {
 }
 #pop-options
 
-instance dh_crypto_invs = {
+instance dh_crypto_invs: crypto_invariants = {
   usages = dh_crypto_usages;
   preds = dh_crypto_preds;
 }
 
 (*** Proofs ***)
+
+val compute_message1_proof:
+  tr:trace ->
+  alice:principal -> bob:principal -> x:bytes -> si:nat ->
+  Lemma
+    (requires
+      event_triggered tr alice (Initiate1 alice bob x) /\
+      is_secret (principal_state_label alice si) tr x /\
+      DhKey? (get_usage x)
+    )
+    (ensures is_publishable tr (compute_message1 alice x))
+let compute_message1_proof tr alice bob x si =
+  let gx = dh_pk x in
+  assert(is_publishable tr gx);
+  let msg = Msg1 {alice; gx} in
+  serialize_wf_lemma message (is_publishable tr) msg;
+
+  // The following code is not needed for the prove.
+  // It just shows what we need to show to prove the lemma.
+  let msgb = compute_message1 alice x in 
+  assert(bytes_invariant tr msgb);
+  assert(get_label msgb `can_flow tr` public);
+  assert(is_publishable tr msgb);
+  ()
+
+val decode_message1_proof:
+  tr:trace ->
+  alice:principal -> bob:principal ->
+  msg_bytes:bytes ->
+  Lemma
+  (requires bytes_invariant tr msg_bytes /\
+    is_publishable tr msg_bytes)
+  (ensures (
+    match decode_message1 msg_bytes with
+    | Some msg1 -> (
+      is_publishable tr msg1.gx
+    )
+    | None -> True
+  ))
+let decode_message1_proof tr alice bob msg_bytes =
+  match decode_message1 msg_bytes with
+    | Some msg1 -> (
+      FStar.Classical.move_requires (parse_wf_lemma message (is_publishable tr)) msg_bytes;
+      FStar.Classical.move_requires (parse_wf_lemma message (bytes_invariant tr)) msg_bytes;
+      
+      // Only for debugging purposes
+      assert(bytes_invariant tr msg1.gx);
+      assert(get_label msg1.gx `can_flow tr` public);
+      ()
+    )
+    | None -> ()
+
+val compute_message2_proof:
+  tr:trace -> si:nat ->
+  alice:principal -> bob:principal ->
+  msg1:message1 ->
+  gy:bytes -> y:bytes ->
+  sk_b:bytes -> n_sig:bytes ->
+  Lemma
+  (requires
+    event_triggered tr bob (Respond1 bob alice msg1.gx gy y) /\
+    is_publishable tr msg1.gx /\ is_publishable tr gy /\
+    is_secret (principal_state_label bob si) tr y /\
+    is_signature_key "DH.SigningKey" (principal_label bob) tr sk_b /\
+    is_secret (principal_label bob) tr n_sig /\
+    SigNonce? (get_usage n_sig)
+  )
+  (ensures
+    is_publishable tr (compute_message2 alice bob msg1.gx gy sk_b n_sig)
+  )
+let compute_message2_proof tr si alice bob msg1 gy y sk_b n_sig =
+  let sig_msg = SigMsg2 {a=alice; gx=msg1.gx; gy} in
+  serialize_wf_lemma sig_message (is_publishable tr) sig_msg;
+  let sig_msg_bytes = serialize sig_message sig_msg in
+  assert(is_publishable tr sig_msg_bytes);
+  let sg = sign sk_b n_sig sig_msg_bytes in
+  
+  assert(bytes_invariant tr sk_b);
+  assert(bytes_invariant tr n_sig);
+  assert(bytes_invariant tr (serialize sig_message sig_msg));
+  assume(SigKey? (get_signkey_usage (Vk sk_b)));
+  assume(dh_crypto_invs.preds.sign_pred tr (Vk sk_b) sig_msg_bytes);
+  assert(SigNonce? (get_usage n_sig));
+  assert((get_label sig_msg_bytes) `can_flow tr` (get_label n_sig));
+
+  assume((get_label sk_b) `can_flow tr` public);
+  assume((get_label n_sig) `can_flow tr` public);
+  assert((get_label sig_msg_bytes) `can_flow tr` public);
+  
+  assume(bytes_invariant tr sg);
+
+  assert(is_publishable tr sg);
+  let msg = Msg2 {bob; gy; sg} in
+  serialize_wf_lemma message (is_publishable tr) msg;
+
+  let msg_bytes = compute_message2 alice bob msg1.gx gy sk_b n_sig in
+  assert(bytes_invariant tr msg_bytes);
+  ()
